Thorough revision in new format. Removed widows and orphans, used new countdown notation, cleaned up codebase and added testing and extracting instructions, incorporated minor catches by reviewers, removed cleverref from all places.

inv_ack.v
@@ -24,7 +24,7 @@ Require Import applications.
    At the end, we also sketch a naive approach to the inverse Ackermann function,
    which uses brute force search, and a massive improvement over it, but still slower
    than our main method for inv_ack, although we do not prove it at the moment
-*)
+ *)
 
 (* *********** INVERSE ACKERMANN HIERARCHY ******************* *)
 
@@ -41,21 +41,21 @@ Theorem alpha_correct :
             upp_inv_rel (alpha m) (ackermann m).
 Proof.
   induction m.
-  { split.
-    - split; intro x; simpl; omega.
-    - intros n x. simpl. omega. }
-  destruct IHm as [IHm0 IHm1]. split.
-  - simpl. split; intro n;
-             rewrite countdown_antirecursion by apply IHm0;
-             apply (countdown_contract_strict 1 _ 1) in IHm0;
-             destruct IHm0 as [IHm00 IHm01]; trivial.
-    + specialize (IHm00 n). omega.
-    + specialize (IHm01 n). omega.
-  - intros n x. simpl. rewrite repeater_from_repeat.
-    rewrite <- repeat_S_comm.
-    apply (upp_inv_repeat (S n) _ _) in IHm1.
-    rewrite <- (IHm1 1 x), repeat_S_comm.
-    apply countdown_repeat. apply IHm0.
+  - split.
+    + split; intro; simpl; omega.
+    + intros n x; simpl; omega. 
+  -  destruct IHm as [IHm0 IHm1]. split.
+     + simpl. split; intro n;
+                rewrite countdown_antirecursion by apply IHm0;
+                apply (countdown_contract_strict 1 _ 1) in IHm0;
+                destruct IHm0 as [IHm00 IHm01]; trivial.
+       * specialize (IHm00 n). omega.
+       * specialize (IHm01 n). omega.
+     + intros n x. simpl. rewrite repeater_from_repeat.
+       rewrite <- repeat_S_comm.
+       apply (upp_inv_repeat (S n) _ _) in IHm1.
+       rewrite <- (IHm1 1 x), repeat_S_comm.
+       now apply countdown_repeat.
 Qed.
 
 
@@ -65,15 +65,15 @@ Qed.
 Lemma ack_repeatable : forall i, repeatable_from 0 (ackermann i).
 Proof.
   induction i; split; try split;
-  intro n; try intro m; simpl; try omega;
-  apply (repeatable_monotone 0 1 _) in IHi; try omega;
-  repeat rewrite repeater_from_repeat;
-  repeat rewrite <- repeat_S_comm;
-  repeat rewrite <- repeater_from_repeat;
-  apply (repeater_repeatable _ 0 _) in IHi; try omega;
-  destruct IHi as [IHi0 IHi1];
-  [intro; apply IHi0; omega | |];
-  apply (Nat.le_trans _ (S (S n)) _); try apply IHi1; omega.
+    intro n; try intro m; simpl; try omega;
+      apply (repeatable_monotone 0 1 _) in IHi; try omega;
+        repeat rewrite repeater_from_repeat;
+        repeat rewrite <- repeat_S_comm;
+        repeat rewrite <- repeater_from_repeat;
+        apply (repeater_repeatable _ 0 _) in IHi; try omega;
+          destruct IHi as [IHi0 IHi1];
+          [intro; apply IHi0; omega | |];
+          apply (Nat.le_trans _ (S (S n)) _); try apply IHi1; omega.
 Qed.
 
 (* Ackermann at level 1. It is useful for 2 purposes:
@@ -88,48 +88,50 @@ Qed.
 (* Alpha at level 1. Used in hard-coding the second level for linear runtime *)
 Lemma alpha_1 : alpha 1 = (fun n => n - 2).
 Proof.
-  assert (upp_inv_rel (alpha 1) (ackermann 1)) as H by apply alpha_correct.
-  assert (upp_inv_rel (fun n => n - 2) (ackermann 1)) as H'.
-  { intros n m. rewrite ack_1. omega. }
-  rewrite upp_inv_unique in H by
-   (intros n m; repeat rewrite ack_1; omega).
-  rewrite upp_inv_unique in H' by
-   (intros n m; repeat rewrite ack_1; omega).
-  rewrite H'. apply H.
+  assert (upp_inv_rel (alpha 1) (ackermann 1)) as H
+      by apply alpha_correct.
+  assert (upp_inv_rel (fun n => n - 2) (ackermann 1)) as H'
+      by (intros n m; rewrite ack_1; omega). 
+  rewrite upp_inv_unique in H
+    by (intros n m; repeat rewrite ack_1; omega).
+  rewrite upp_inv_unique in H'
+    by (intros n m; repeat rewrite ack_1; omega).
+  now rewrite H'. 
 Qed.
 
-(* Below two results asserts that the diagonal Ackermann function is increasing,
-   hence has a proper upper inverse. We need them because we need to compute the inverse
+(* The two results below show that the diagonal Ackermann function is increasing,
+   and therefore has a proper upper inverse. We need them because we need to compute the inverse
    value for the inv_ack correctness proof later *)
 
 (* Strict Increasing With Level *)
 Lemma ack_incr_by_lvl :
-    forall n, increasing (fun i => ackermann i n).
+  forall n, increasing (fun i => ackermann i n).
 Proof.
   intro n. rewrite incr_S. intro i. generalize dependent n.
   induction i; intro n.
-  - rewrite ack_1. simpl. omega.
-  - remember (S i) as p. destruct n.
-    + simpl. apply ack_repeatable. omega.
-    + rewrite ackermann_recursion. apply ack_repeatable.
-      assert (Hi := IHi).
-      rewrite Heqp in IHi. specialize (IHi (S n)).
-      rewrite ackermann_recursion in IHi.
-      rewrite <- incr_twoways in IHi by apply ack_repeatable.
-      apply (Nat.lt_trans _ (ackermann (S i) n) _); trivial.
-      clear IHi. induction n.
-      * simpl. apply Hi.
-      * repeat rewrite ackermann_recursion.
-        apply (Nat.lt_trans _ (ackermann i (ackermann (S p) n)) _).
-        apply ack_repeatable; assumption.
-        apply Hi.
+  1: rewrite ack_1; simpl; omega.
+  remember (S i) as p. destruct n.
+  1: simpl; apply ack_repeatable; omega.
+  rewrite ackermann_recursion. apply ack_repeatable.
+  assert (Hi := IHi).
+  rewrite Heqp in IHi. specialize (IHi (S n)).
+  rewrite ackermann_recursion in IHi.
+  rewrite <- incr_twoways in IHi by apply ack_repeatable.
+  apply (Nat.lt_trans _ (ackermann (S i) n) _); trivial.
+  clear IHi. induction n.
+  1: simpl; easy.
+  repeat rewrite ackermann_recursion.
+  apply (Nat.lt_trans _ (ackermann i (ackermann (S p) n)) _).
+  apply ack_repeatable; assumption.
+  apply Hi.
 Qed.
 
 (* Diagonal Strict Increasing *)
 Lemma diag_ack_incr : increasing (fun n => ackermann n n).
 Proof.
-  intros n m Hnm. apply (Nat.lt_trans _ (ackermann n m) _);
-  [apply ack_repeatable| apply ack_incr_by_lvl]; assumption.
+  intros n m Hnm.
+  apply (Nat.lt_trans _ (ackermann n m) _);
+    [apply ack_repeatable | apply ack_incr_by_lvl]; assumption.
 Qed.
 
 
@@ -138,65 +140,65 @@ Qed.
 Fixpoint inv_ack_worker (f : nat -> nat) (n k bud : nat) : nat :=
   match bud with
   | 0      => k
-  | S bud' =>
-    match (n - k) with
-    | 0   => k
-    | S _ =>
-      let g := (countdown_to f 1) in
-      inv_ack_worker (compose g f) (g n) (S k) bud'
-    end
+  | S bud' => match (n - k) with
+              | 0   => k
+              | S _ => let g := (countdown_to f 1) in
+                       inv_ack_worker (compose g f) (g n) (S k) bud'
+              end
   end.
 
 (* Original defintion, runtime O(n^2) *)
-Definition inv_ack n :=
-  match (alpha 0) with f => inv_ack_worker f (f n) 0 n end.
+Definition inv_ack n := inv_ack_worker (alpha 0) (alpha 0 n) 0 n.
 
 (* Intermediate lemma about inv_ack_worker *)
 Lemma inv_ack_worker_intermediate :
-    forall i n b, (i < alpha i n) -> (i < b) ->
-        (inv_ack_worker (alpha 0) (alpha 0 n) 0 b
-         = inv_ack_worker (alpha (S i)) (alpha (S i) n) (S i) (b - (S i))).
-    induction i.
-    - simpl. intros n b Hn Hb. unfold inv_ack_worker.
-      destruct b; try omega.
-      remember ((n - 1) - 0) as m. destruct m; try omega.
-      replace (S b - 1) with b by omega. trivial.
-    - intros n b Hn Hb. rewrite IHi.
-      + remember (S i) as p.
-        replace (alpha (S p)) with
-        (compose (countdown_to (alpha p) 1) (alpha p)) by trivial.
-        unfold inv_ack_worker.
-        remember (alpha p n - p) as m. destruct m; try omega.
-        remember (b - p) as c. destruct c; try omega.
-        replace (b - S p) with c by omega.
-        rewrite <- Heqm. trivial.
-      + rewrite <- not_le. destruct (alpha_correct i) as [_ Halphai].
-        rewrite (Halphai i n). intro.
-        assert (n <= ackermann (S i) (S i)).
-        { apply (Nat.le_trans _ (ackermann i i) _); trivial.
-          apply Nat.lt_le_incl. apply diag_ack_incr. omega. }
-        destruct (alpha_correct (S i)) as [_ HalphaSi].
-        rewrite <- (HalphaSi (S i) n) in H0. omega.
-      + omega.
+  forall i n b,
+    i < alpha i n ->
+    i < b ->
+    inv_ack_worker (alpha 0) (alpha 0 n) 0 b =
+    inv_ack_worker (alpha (S i)) (alpha (S i) n) (S i) (b - (S i)).
+  induction i.
+  - simpl. intros n b Hn Hb. unfold inv_ack_worker.
+    destruct b; try omega.
+    remember ((n - 1) - 0) as m. destruct m; try omega.
+    replace (S b - 1) with b by omega. trivial.
+  - intros n b Hn Hb. rewrite IHi.
+    + remember (S i) as p.
+      replace (alpha (S p)) with (compose (countdown_to (alpha p) 1) (alpha p))
+        by trivial.
+      unfold inv_ack_worker.
+      remember (alpha p n - p) as m. destruct m; try omega.
+      remember (b - p) as c. destruct c; try omega.
+      replace (b - S p) with c by omega.
+      rewrite <- Heqm. trivial.
+    + rewrite <- not_le. destruct (alpha_correct i) as [_ Halphai].
+      rewrite (Halphai i n). intro.
+      assert (n <= ackermann (S i) (S i)).
+      { apply (Nat.le_trans _ (ackermann i i) _); trivial.
+        apply Nat.lt_le_incl. apply diag_ack_incr. omega. }
+      destruct (alpha_correct (S i)) as [_ HalphaSi].
+      rewrite <- (HalphaSi (S i) n) in H0. omega.
+    + omega.
 Qed.
 
-(* Proof that inv_ack is correct *)
+
+(* Proof that inv_ack correctly calculates the inverse of the diagonal Ackermann-Peter function *)
 Theorem inv_ack_correct :
   upp_inv_rel inv_ack (fun k => ackermann k k).
 Proof.
   rewrite upp_inv_unique by apply diag_ack_incr.
   assert (forall n N : nat,
-            upp_inv (fun k : nat => ackermann k k) N <= n
-            <-> alpha n N <= n) as H.
+             upp_inv (fun k : nat => ackermann k k) N <= n
+             <-> alpha n N <= n) as H.
   { intros n N.
     rewrite (upp_inv_correct (fun k : nat => ackermann k k)
-           diag_ack_incr n N). destruct (alpha_correct n) as [_ Hm].
+                             diag_ack_incr n N). destruct (alpha_correct n) as [_ Hm].
     symmetry. apply Hm. }
   apply functional_extensionality. intro n.
   remember (upp_inv (fun k : nat => ackermann k k) n) as m.
   unfold inv_ack. assert (H0 := H). destruct m.
   - specialize (H 0 n). rewrite <- Heqm in H.
-    assert (n <= 1) as Hn. { simpl in H. omega. }
+    assert (n <= 1) as Hn by (simpl in H; omega). 
     destruct n; simpl; trivial; destruct n; simpl; trivial; omega.
   - specialize (H m n). rewrite <- Heqm in H.
     assert (m < alpha m n) as Hn by omega.
@@ -207,93 +209,63 @@ Proof.
       destruct (ack_repeatable m) as [_ Hackm].
       destruct Hackm as [_ Hackm]. specialize (Hackm m).
       omega. }
-    rewrite (inv_ack_worker_intermediate m n n).
-    assert (alpha (S m) n - (S m) = 0).
-    { specialize (H0 (S m) n). rewrite <- Heqm in H0. omega. }
+    rewrite (inv_ack_worker_intermediate m n n Hn).
+    2: omega.
+    assert (alpha (S m) n - (S m) = 0)
+      by (specialize (H0 (S m) n); rewrite <- Heqm in H0; omega).
     unfold inv_ack_worker.
-    remember (n - S m) as p. destruct p; try omega.
-    + rewrite H1. trivial.
-    + assumption.
-    + omega.
+    remember (n - S m) as p. destruct p; try omega. 
+    rewrite H1. trivial.
 Qed.
 
 (* ****** INVERSE ACKERMANN BY HARD-CODING SECOND LEVEL ************* *)
 
 (* Definition by hard-coding the second alpha level, runtime O(n) *)
-Definition inv_ack' n :=
+Definition inv_ack_linear n :=
   match n with
   | 0 | 1 => 0
   | _     => match (fun x => x - 2) with f
-             => inv_ack_worker f (f n) 1 (n - 1) end
+                                         => inv_ack_worker f (f n) 1 (n - 1) end
   end.
 
 (* Correctness proof *)
-Theorem inv_ack'_correct : inv_ack' = inv_ack.
+Theorem inv_ack_linear_correct : inv_ack_linear = inv_ack.
 Proof.
   apply functional_extensionality. intro n.
-  unfold inv_ack. unfold inv_ack'.
+  unfold inv_ack, inv_ack_linear.
   destruct n; try destruct n; trivial.
   rewrite (inv_ack_worker_intermediate 0 _ _) by (simpl; omega).
-  rewrite alpha_1. trivial.
+  rewrite alpha_1; trivial.
 Qed.
 
+(* Demonstrating Linear Runtime *)
+Time Compute inv_ack_linear 10000.
+Time Compute inv_ack_linear 100000.
+Time Compute inv_ack_linear 1000000.
+Time Compute inv_ack_linear 10000000.
 
-(* *********** NAIVE INVERSE ACKERMANN FUNCTION ******************** *)
-
-Fixpoint inv_ack_naive (n : nat) (ans : nat) (bud : nat) : nat :=
-  match bud with
-  | 0 => 0
-  | S bud' =>
-    match n - (ackermann ans ans) with
-    | 0 => ans
-    | _ => inv_ack_naive n (S ans) bud'
-    end
-  end.
-
-Definition inv_ack_naive_outer n := inv_ack_naive n 0 n.
-
-(* Compute inv_ack_naive_outer 62. *)
-(* Obviously this gets busy calculating A(4). *)
-
-(* So let's try to do better: 
-   Stop calculating A(4) the moment the "rolling answer" blows past n.
-   This works out well because Ackermann grows monotonically even _within_ the calculation of a single term.
- *)
-
+(* Our code can be extracted to OCaml by running the two lines below: *)
 (* 
- * Here we have a tail-recursive variant of repeater_from, 
- * with an added feature: 
- * If we cross the "target", we stop and return 
- * our working answer 
+Require Extraction. 
+Recursive Extraction inv_ack_linear.
 *)
-Fixpoint repeater_from_tail_target ans f n target : nat :=
-  match target - ans with
-  | 0 => ans
-  | _ =>
-    match n with
-    | 0 => ans
-    | S n' => repeater_from_tail_target (f ans) f n' target
-    end
-  end.
 
-Fixpoint ackermann_target target m n :=
-  match m with
-  | 0 => S n
-  | S m' => repeater_from_tail_target (ackermann_target target m' 1) (ackermann_target target m') n target
-  end.
+(* Next, our benchmarks can be tested in OCaml as follows: *)
+(*
+let time n f x =
+    let t = Sys.time() in
+    let ans = f x in
+    Printf.printf "Execution time for %d: \t%fs\n" n (Sys.time() -. t); ans;;
 
-(* Compute ackermann_target 70 4 4. *)
-(* --> returns 70 immediately. Because it is not
-   concerned with actually calculating A(4,4). *)
+let rec buildnat j acc = 
+  if j = 0 then acc else buildnat (j-1) (S acc);;
 
-Fixpoint inv_ack_target (n : nat) (ans : nat) (bud : nat) : nat :=
-  match bud with
-  | 0 => 0
-  | S bud' =>
-    match (n - (ackermann_target n ans ans)) with
-    | 0 => ans
-    | _ => inv_ack_target n (ans + 1) (bud')
-    end
-  end.
+let time_print n = 
+  time n inv_ack_linear (buildnat n O);;
 
-Definition inv_ack_target_outer n := inv_ack_target n 0 n.
+time_print 100;;
+time_print 1000;;
+time_print 10000;;
+time_print 100000;;
+time_print 1000000;;
+*)
